store/server_proofs/store.v
@@ -30,7 +30,7 @@ Variable N : namespace.
 Lemma wp_server_handle_store c kI kR cs (vdb : val) :
   {{{ channel c ∗ cryptis_ctx ∗ store_ctx N }}}
     RPC.handle N "store" c (Server.handle_store c (repr cs) vdb)
-  {{{ h, RET h; server_handler N kI kR cs vdb h }}}.
+  {{{ h, RET (repr h); server_handler N kI kR cs vdb h }}}.
 Proof.
 iIntros "%Φ (#chan_c & #? & #ctx) post".
 iPoseProof (store_ctx_store with "ctx") as "?".
